Shortened the proofs HP.thy

2026-NMR-CKM/HP.thy
@@ -3,127 +3,98 @@ theory HP
   imports Main Helper
 begin
 
-text \<open>Shallow embedding of single-world causal models in HOL.\<close>
+text ‹Shallow embedding of single-world causal models in HOL.›
 
-text \<open>Type declarations\<close>
-typedecl \<v>  (* Causal variables *)
-typedecl \<iota>  (* Individuals *)
+text ‹Type declarations›
+typedecl 𝗏  (* Causal variables *)
+typedecl ι  (* Individuals *)
 
-type_synonym \<X> = "\<v> \<Rightarrow> bool"              (* Sets of causal variables *)
-type_synonym \<R> = "\<v> \<Rightarrow> (\<iota> \<Rightarrow> bool)" (* Ranges of variables *)
-type_synonym \<f> = "(\<v> \<Rightarrow> \<iota>) \<Rightarrow> \<iota>" (* Structural equations *)
-type_synonym \<F> = "\<v> \<Rightarrow> \<f>"               (* Families of structural equations *)
-type_synonym \<t> = "\<v> \<Rightarrow> \<iota>"             (* Total assignments / contexts *)
+type_synonym 𝒳 = "𝗏 ⇒ bool"              (* Sets of causal variables *)
+type_synonym ℛ = "𝗏 ⇒ (ι ⇒ bool)" (* Ranges of variables *)
+type_synonym 𝖿 = "(𝗏 ⇒ ι) ⇒ ι" (* Structural equations *)
+type_synonym ℱ = "𝗏 ⇒ 𝖿"               (* Families of structural equations *)
+type_synonym 𝗍 = "𝗏 ⇒ ι"             (* Total assignments / contexts *)
 
-(* Keeping only one formula type. The old \<alpha>-layer is redundant in this shallow embedding.
-   type_synonym \<alpha> = "\<F> \<Rightarrow> bool" *)
-type_synonym \<Phi>   = "\<F> \<Rightarrow> bool"
+type_synonym Φ   = "ℱ ⇒ bool"
 
 consts
-  U  :: \<X>    (* Exogenous variables *)
-  V  :: \<X>    (* Endogenous variables *)
-  F  :: \<F>    (* Initial structural family *)
-  R  :: \<R>    (* Ranges *)
-  tx :: \<t>    (* Actual exogenous context *)
+  U  :: 𝒳    (* Exogenous variables *)
+  V  :: 𝒳    (* Endogenous variables *)
+  F  :: ℱ    (* Initial structural family *)
+  R  :: ℛ    (* Ranges *)
+  tx :: 𝗍    (* Actual exogenous context *)
 
-text \<open>
-  y directly depends on x if changing x while keeping the rest of an assignment fixed
-  can change the value produced by the equation for y.
-\<close>
-abbreviation (input) directly_depends :: "\<v> \<Rightarrow> \<f> \<Rightarrow> \<X>" where
-  "directly_depends y f \<equiv>
-     \<lambda>x. \<exists>i1 i2 Z. x \<noteq> y \<and> i1 \<noteq> i2 \<and> R x i1 \<and> R x i2 \<and>
-          f (fun_upd Z x i1) \<noteq> f (fun_upd Z x i2)"
+abbreviation (input) directly_depends :: "𝗏 ⇒ 𝖿 ⇒ 𝒳" where
+  "directly_depends y f ≡
+     λx. ∃i1 i2 Z. x ≠ y ∧ i1 ≠ i2 ∧ R x i1 ∧ R x i2 ∧
+          f (fun_upd Z x i1) ≠ f (fun_upd Z x i2)"
 
-definition directly_causes :: "\<F> \<Rightarrow> (\<v> \<Rightarrow> \<v> \<Rightarrow> bool)" where
-  "directly_causes G \<equiv> \<lambda>x v. directly_depends v (G v) x"
+definition directly_causes :: "ℱ ⇒ (𝗏 ⇒ 𝗏 ⇒ bool)" where
+  "directly_causes G ≡ λx v. directly_depends v (G v) x"
 
 axiomatization where
-  disjoint_variables: "\<forall>x. U x \<longleftrightarrow> \<not> V x" and
-  exo: "\<forall>x a. U x \<longrightarrow> F x a = tx x" and
-  equations_respect_ranges: "\<forall>v t. R v (F v t)" and
-  tx_respects_F: "\<forall>v. F v tx = tx v" and
+  disjoint_variables: "∀x. U x ⟷ ¬ V x" and
+  exo: "∀x a. U x ⟶ F x a = tx x" and
+  equations_respect_ranges: "∀v t. R v (F v t)" and
+  tx_respects_F: "∀v. F v tx = tx v" and
   depends_only_on_direct_causes:
-    "\<forall>v a1 a2. (\<forall>x. directly_depends v (F v) x \<longrightarrow> a1 x = a2 x) \<longrightarrow> F v a1 = F v a2"
+    "∀v a1 a2. (∀x. directly_depends v (F v) x ⟶ a1 x = a2 x) ⟶ F v a1 = F v a2"
 
-lemma tx_respects_ranges:
-  "\<forall>v. R v (tx v)"
+lemma tx_respects_ranges: "∀v. R v (tx v)"
   by (metis equations_respect_ranges tx_respects_F)
 
-lemma nonempty_ranges:
-  "\<forall>v. \<exists>i. R v i"
+lemma nonempty_ranges: "∀v. ∃i. R v i"
   using tx_respects_ranges by auto
 
 lemma no_self_dependence:
-  "\<forall>v a1 a2. (\<forall>w. w \<noteq> v \<longrightarrow> a1 w = a2 w) \<longrightarrow> F v a1 = F v a2"
+  "∀v a1 a2. (∀w. w ≠ v ⟶ a1 w = a2 w) ⟶ F v a1 = F v a2"
   using depends_only_on_direct_causes by blast
 
-lemma exo_no_direct_dep:
-  "\<forall>x v. U v \<longrightarrow> \<not> directly_depends v (F v) x"
+lemma exo_no_direct_dep: "∀x v. U v ⟶ ¬ directly_depends v (F v) x"
   by (simp add: exo)
 
-text \<open>Fixed-point view of solutions.\<close>
-definition next_ctx :: "\<F> \<Rightarrow> \<t> \<Rightarrow> \<t>" where
-  "next_ctx G ctx \<equiv> (\<lambda>v. if U v then tx v else G v ctx)"
+text ‹Fixed-point view of solutions.›
+definition next_ctx :: "ℱ ⇒ 𝗍 ⇒ 𝗍" where
+  "next_ctx G ctx ≡ (λv. if U v then tx v else G v ctx)"
 
-definition Fix :: "\<F> \<Rightarrow> \<t> \<Rightarrow> bool" where
-  "Fix G ctx \<equiv> next_ctx G ctx = ctx"
+definition Fix :: "ℱ ⇒ 𝗍 ⇒ bool" where
+  "Fix G ctx ≡ next_ctx G ctx = ctx"
 
 lemma Fix_iff_solution:
-  "Fix G ctx \<longleftrightarrow>
-     (\<forall>u. U u \<longrightarrow> ctx u = tx u) \<and> (\<forall>v. V v \<longrightarrow> ctx v = G v ctx)"
+  "Fix G ctx ⟷
+     (∀u. U u ⟶ ctx u = tx u) ∧ (∀v. V v ⟶ ctx v = G v ctx)"
   by (metis (lifting) Fix_def disjoint_variables ext next_ctx_def)
 
-text \<open>A fixed topological order for the initial family F.\<close>
-consts ord :: "\<v> list"
+text ‹A fixed topological order for the initial family F.›
+consts ord :: "𝗏 list"
 
 axiomatization where
   ord_distinct: "distinct ord" and
   ord_complete: "set ord = {v. V v}" and
-  topo_ord: "directly_causes F x v \<Longrightarrow> U x \<or> find_index ord x < find_index ord v"
-
-text \<open>
-  We take the list ord as the only structural order notion.
-  Recursiveness is expressed directly by ord; no separate auxiliary order relation is introduced.
-\<close>
-
-(* endo_not_leaves: intentionally not assumed.
-   Recursive models may have endogenous roots, e.g. variables that depend only on exogenous inputs. *)
+  topo_ord: "directly_causes F x v ⟹ U x ∨ find_index ord x < find_index ord v"
 
 lemma recur_ord:
-  "\<forall>x v. x \<noteq> v \<longrightarrow>
-      ((U x \<and> V v) \<or> (V x \<and> V v \<and> find_index ord x < find_index ord v)) \<longrightarrow>
-      \<not> ((U v \<and> V x) \<or> (V v \<and> V x \<and> find_index ord v < find_index ord x))"
+  "∀x v. x ≠ v ⟶
+      ((U x ∧ V v) ∨ (V x ∧ V v ∧ find_index ord x < find_index ord v)) ⟶
+      ¬ ((U v ∧ V x) ∨ (V v ∧ V x ∧ find_index ord v < find_index ord x))"
   by (metis disjoint_variables less_irrefl less_trans)
 
-text \<open>
-  Constructive solver: traverse the endogenous variables in the fixed order ord,
-  updating the current assignment with the value given by the current equation family.
-\<close>
-definition step_ctx :: "\<F> \<Rightarrow> \<t> \<Rightarrow> \<v> \<Rightarrow> \<t>" where
-  "step_ctx G c v \<equiv> fun_upd c v (G v c)"
+definition step_ctx :: "ℱ ⇒ 𝗍 ⇒ 𝗏 ⇒ 𝗍" where
+  "step_ctx G c v ≡ fun_upd c v (G v c)"
 
-definition cv :: "\<F> \<Rightarrow> \<t>" where
-  "cv G \<equiv> foldl (step_ctx G) tx ord"
+definition cv :: "ℱ ⇒ 𝗍" where
+  "cv G ≡ foldl (step_ctx G) tx ord"
 
 lemma foldl_step_notin:
-  assumes "x \<notin> set xs"
+  assumes "x ∉ set xs"
   shows "foldl (step_ctx G) c xs x = c x"
   using assms
 proof (induction xs arbitrary: c)
-  case Nil
-  then show ?case by simp
+  case Nil then show ?case by simp
 next
   case (Cons a xs)
-  have xa: "x \<noteq> a" and xxs: "x \<notin> set xs"
-    using Cons.prems by auto
-  have "foldl (step_ctx G) c (a # xs) x = foldl (step_ctx G) (step_ctx G c a) xs x"
-    by simp
-  also have "... = step_ctx G c a x"
-    using Cons.IH[OF xxs] by simp
-  also have "... = c x"
-    using xa unfolding step_ctx_def by simp
-  finally show ?case .
+  have "x ≠ a" and "x ∉ set xs" using Cons.prems by auto
+  then show ?case using Cons.IH step_ctx_def by force
 qed
 
 lemma cv_exo [simp]:
@@ -134,280 +105,198 @@ lemma cv_exo [simp]:
 lemma index_at_split [simp]:
   assumes dist: "distinct (prefix @ v # suffix)"
   shows "find_index (prefix @ v # suffix) v = length prefix"
-proof -
-  have mem: "v \<in> set (prefix @ v # suffix)"
-    by simp
-  have lt1: "find_index (prefix @ v # suffix) v < length (prefix @ v # suffix)"
-    using find_index_lt_length_if_mem[OF mem] .
-  have nth1: "(prefix @ v # suffix) ! find_index (prefix @ v # suffix) v = v"
-    using find_index_nth_if_mem[OF mem] .
-  have lt2: "length prefix < length (prefix @ v # suffix)"
-    by simp
-  have nth2: "(prefix @ v # suffix) ! length prefix = v"
-    by simp
-  from dist lt1 lt2 nth1 nth2 show ?thesis
-    by (metis distinct_conv_nth)
-qed
+  by (metis add_less_cancel_left append.right_neutral dist distinct_Ex1 find_index_lt_length_if_mem 
+         find_index_nth_if_mem length_Cons length_append list.size(3) nth_append_length nth_mem zero_less_Suc)
 
-text \<open>Language\<close>
+text ‹Language›
 
-(* Redundant \<alpha>-layer kept only as a comment.
-   definition AtomAlpha :: "\<v> \<Rightarrow> \<iota> \<Rightarrow> \<alpha>" ("_=\<^sup>h\<^sup>p\<^sup>a_") where
-     "v =\<^sup>h\<^sup>p\<^sup>a i \<equiv> \<lambda>G. V v \<and> R v i \<and> cv G v = i"
-   definition NegationAlpha :: "\<alpha> \<Rightarrow> \<alpha>" ("\<not>\<^sup>h\<^sup>p\<^sup>a") where
-     "\<not>\<^sup>h\<^sup>p\<^sup>a \<phi> \<equiv> \<lambda>G. \<not> \<phi> G"
-   definition ConjunctionAlpha :: "\<alpha> \<Rightarrow> \<alpha> \<Rightarrow> \<alpha>" (infixr "\<and>\<^sup>h\<^sup>p\<^sup>a" 95) where
-     "\<phi> \<and>\<^sup>h\<^sup>p\<^sup>a \<psi> \<equiv> \<lambda>G. \<phi> G \<and> \<psi> G"
-   definition ImplicationAlpha :: "\<alpha> \<Rightarrow> \<alpha> \<Rightarrow> \<alpha>" (infixr "\<rightarrow>\<^sup>h\<^sup>p\<^sup>a" 95) where
-     "\<phi> \<rightarrow>\<^sup>h\<^sup>p\<^sup>a \<psi> \<equiv> \<lambda>G. \<phi> G \<longrightarrow> \<psi> G" *)
+definition AtomPhi :: "𝗏 ⇒ ι ⇒ Φ" ("_=⇧h⇧p⇧p_") where
+  "v =⇧h⇧p⇧p i ≡ λG. V v ∧ R v i ∧ cv G v = i"
 
-definition AtomPhi :: "\<v> \<Rightarrow> \<iota> \<Rightarrow> \<Phi>" ("_=\<^sup>h\<^sup>p\<^sup>p_") where
-  "v =\<^sup>h\<^sup>p\<^sup>p i \<equiv> \<lambda>G. V v \<and> R v i \<and> cv G v = i"
+definition NegationPhi :: "Φ ⇒ Φ" ("¬⇧h⇧p⇧p") where
+  "¬⇧h⇧p⇧p φ ≡ λG. ¬ φ G"
 
-definition NegationPhi :: "\<Phi> \<Rightarrow> \<Phi>" ("\<not>\<^sup>h\<^sup>p\<^sup>p") where
-  "\<not>\<^sup>h\<^sup>p\<^sup>p \<phi> \<equiv> \<lambda>G. \<not> \<phi> G"
+definition ConjunctionPhi :: "Φ ⇒ Φ ⇒ Φ" (infixr "∧⇧h⇧p⇧p" 95) where
+  "φ ∧⇧h⇧p⇧p ψ ≡ λG. φ G ∧ ψ G"
 
-definition ConjunctionPhi :: "\<Phi> \<Rightarrow> \<Phi> \<Rightarrow> \<Phi>" (infixr "\<and>\<^sup>h\<^sup>p\<^sup>p" 95) where
-  "\<phi> \<and>\<^sup>h\<^sup>p\<^sup>p \<psi> \<equiv> \<lambda>G. \<phi> G \<and> \<psi> G"
+definition ImplicationPhi :: "Φ ⇒ Φ ⇒ Φ" (infixr "→⇧h⇧p⇧p" 95) where
+  "φ →⇧h⇧p⇧p ψ ≡ λG. φ G ⟶ ψ G"
 
-definition ImplicationPhi :: "\<Phi> \<Rightarrow> \<Phi> \<Rightarrow> \<Phi>" (infixr "\<rightarrow>\<^sup>h\<^sup>p\<^sup>p" 95) where
-  "\<phi> \<rightarrow>\<^sup>h\<^sup>p\<^sup>p \<psi> \<equiv> \<lambda>G. \<phi> G \<longrightarrow> \<psi> G"
+definition wf_intervention :: "𝗏 ⇒ ι ⇒ bool" where
+  "wf_intervention v i ≡ V v ∧ R v i"
 
-text \<open>Pointwise well-formedness for a single intervention target/value pair.\<close>
-definition wf_intervention :: "\<v> \<Rightarrow> \<iota> \<Rightarrow> bool" where
-  "wf_intervention v i \<equiv> V v \<and> R v i"
-
-lemma wf_intervention_iff [simp]:
-  "wf_intervention v i \<longleftrightarrow> V v \<and> R v i"
+lemma wf_intervention_iff [simp]: "wf_intervention v i ⟷ V v ∧ R v i"
   unfolding wf_intervention_def by simp
 
-text \<open>
-  Intervention replaces selected structural equations by constants.
-  The well-formedness check is internalized pointwise in update_F.
-\<close>
-definition update_F :: "\<F> \<Rightarrow> \<X> \<Rightarrow> (\<v> \<Rightarrow> \<iota>) \<Rightarrow> \<F>" where
-  "update_F G Y b \<equiv> \<lambda>v a. if Y v \<and> wf_intervention v (b v) then b v else G v a"
+definition update_F :: "ℱ ⇒ 𝒳 ⇒ (𝗏 ⇒ ι) ⇒ ℱ" where
+  "update_F G Y b ≡ λv a. if Y v ∧ wf_intervention v (b v) then b v else G v a"
 
-definition Intervention :: "\<X> \<Rightarrow> (\<v> \<Rightarrow> \<iota>) \<Rightarrow> \<Phi> \<Rightarrow> \<Phi>" ("[_\<leftarrow>_]_") where
-  "[Y \<leftarrow> b] \<phi> \<equiv> \<lambda>G. \<phi> (update_F G Y b)"
+definition Intervention :: "𝒳 ⇒ (𝗏 ⇒ ι) ⇒ Φ ⇒ Φ" ("[_←_]_") where
+  "[Y ← b] φ ≡ λG. φ (update_F G Y b)"
 
-inductive reachable :: "\<F> \<Rightarrow> bool" where
+inductive reachable :: "ℱ ⇒ bool" where
   reachable_base [intro]: "reachable F" |
-  reachable_step [intro]: "reachable G \<Longrightarrow> reachable (update_F G Y b)"
+  reachable_step [intro]: "reachable G ⟹ reachable (update_F G Y b)"
 
 lemma directly_causes_update_subset [simp]:
   assumes "directly_causes (update_F G Y b) x v"
   shows "directly_causes G x v"
   using assms unfolding directly_causes_def update_F_def by metis
 
-definition Truth :: "\<F> \<Rightarrow> \<Phi> \<Rightarrow> bool" ("\<langle>_\<rangle> \<Turnstile>\<^sup>h\<^sup>p\<^sup>p _") where
-  "\<langle>G\<rangle> \<Turnstile>\<^sup>h\<^sup>p\<^sup>p \<phi> \<equiv> \<phi> G"
+definition Truth :: "ℱ ⇒ Φ ⇒ bool" ("⟨_⟩ ⊨⇧h⇧p⇧p _") where
+  "⟨G⟩ ⊨⇧h⇧p⇧p φ ≡ φ G"
 
-definition Validity ("\<Turnstile>\<^sup>h\<^sup>p\<^sup>p _") where
-  "\<Turnstile>\<^sup>h\<^sup>p\<^sup>p \<phi> \<equiv> \<forall>G. reachable G \<longrightarrow> \<langle>G\<rangle> \<Turnstile>\<^sup>h\<^sup>p\<^sup>p \<phi>"
+definition Validity ("⊨⇧h⇧p⇧p _") where
+  "⊨⇧h⇧p⇧p φ ≡ ∀G. reachable G ⟶ ⟨G⟩ ⊨⇧h⇧p⇧p φ"
 
-lemma reachable_update_F [intro]:
-  "reachable (update_F F Y b)"
+lemma reachable_update_F [intro]: "reachable (update_F F Y b)"
   by (rule reachable_step[OF reachable_base])
 
 lemma reachable_directly_causes_subset_F [simp]:
-  assumes rG: "reachable G" and dc: "directly_causes G x v"
+  assumes "reachable G" and "directly_causes G x v"
   shows "directly_causes F x v"
-  using assms by (induction) auto
+  using assms by induction auto
 
 lemma reachable_respects_ranges [simp]:
   assumes "reachable G"
-  shows "\<forall>v t. R v (G v t)"
-  using assms
-  by (induction) (auto simp: equations_respect_ranges update_F_def)
+  shows "∀v t. R v (G v t)"
+  using assms by (induction) (auto simp: equations_respect_ranges update_F_def)
 
 lemma reachable_exo [simp]:
   assumes "reachable G"
-  shows "\<forall>x a. U x \<longrightarrow> G x a = tx x"
-  using assms
-  by (induction) (auto simp: exo update_F_def disjoint_variables)
+  shows "∀x a. U x ⟶ G x a = tx x"
+  using assms by (induction) (auto simp: exo update_F_def disjoint_variables)
 
 lemma reachable_locality [simp]:
   assumes "reachable G"
-  shows "\<forall>v a1 a2. (\<forall>x. directly_depends v (G v) x \<longrightarrow> a1 x = a2 x) \<longrightarrow> G v a1 = G v a2"
-  using assms 
+  shows "∀v a1 a2. (∀x. directly_depends v (G v) x ⟶ a1 x = a2 x) ⟶ G v a1 = G v a2"
+  using assms
   apply induction
   using depends_only_on_direct_causes apply blast
   by (smt (verit, del_insts) update_F_def)
 
 lemma reachable_topo_index [simp]:
-  assumes rG: "reachable G" and dc: "directly_causes G x v"
-  shows "U x \<or> find_index ord x < find_index ord v"
-  by (metis dc rG reachable_directly_causes_subset_F topo_ord)
+  assumes "reachable G" and "directly_causes G x v"
+  shows "U x ∨ find_index ord x < find_index ord v"
+  by (metis assms reachable_directly_causes_subset_F topo_ord)
 
 lemma cv_reachable_endo [simp]:
   assumes rG: "reachable G" and Vv: "V v"
   shows "cv G v = G v (cv G)"
 proof -
-  from ord_complete Vv have vmem: "v \<in> set ord"
-    by auto
+  from ord_complete Vv have vmem: "v ∈ set ord" by auto
   then obtain prefix suffix where dec: "ord = prefix @ v # suffix"
-    using split_list 
-    by metis
+    using split_list by metis
   let ?cpre = "foldl (step_ctx G) tx prefix"
-  have dist: "distinct (prefix @ v # suffix)"
-    using ord_distinct dec by simp
-  have vnot: "v \<notin> set suffix"
-    using dist by auto
-  have cvv: "cv G v = G v ?cpre" 
-  proof -
-    have "cv G v = foldl (step_ctx G) (step_ctx G ?cpre v) suffix v"
-      unfolding cv_def dec by simp
-    also have "... = step_ctx G ?cpre v v"
-      by (simp add: foldl_step_notin vnot)
-    also have "... = G v ?cpre"
-      unfolding step_ctx_def by simp
-    finally show ?thesis .
-  qed
-  have agree: "\<forall>x. directly_depends v (G v) x \<longrightarrow> ?cpre x = cv G x"
+  have dist: "distinct (prefix @ v # suffix)" using ord_distinct dec by simp
+  have vnot: "v ∉ set suffix" using dist by auto
+  have cvv: "cv G v = G v ?cpre"
+    using foldl_step_notin[OF vnot]
+    by (simp add: cv_def dec step_ctx_def)
+  have agree: "∀x. directly_depends v (G v) x ⟶ ?cpre x = cv G x"
   proof (intro allI impI)
     fix x
     assume dx: "directly_depends v (G v) x"
-    have topo: "U x \<or> find_index ord x < find_index ord v"
-      using reachable_topo_index[OF rG] dx
-      unfolding directly_causes_def by blast
+    have topo: "U x ∨ find_index ord x < find_index ord v"
+      using reachable_topo_index[OF rG] dx unfolding directly_causes_def by blast
     show "?cpre x = cv G x"
     proof (cases "U x")
       case True
-      have xnotpref: "x \<notin> set prefix"
-        using True ord_complete disjoint_variables dec 
+      have xnotpref: "x ∉ set prefix"
+        using True ord_complete disjoint_variables dec
         by (metis append_eq_conv_conj in_set_takeD mem_Collect_eq)
-      have cprex: "?cpre x = tx x"
-        by (simp add: foldl_step_notin xnotpref)
-      have cvx: "cv G x = tx x"
-        using cv_exo[of x G] True by simp
-      show ?thesis
-        using cprex cvx by simp
+      then show ?thesis
+        by (simp add: foldl_step_notin True)
     next
       case False
-      then have Vx: "V x"
-        using disjoint_variables by blast
-      have xmem: "x \<in> set ord"
-        using ord_complete Vx by auto
-      have idx: "find_index ord x < find_index ord v"
-        using topo False by simp
+      then have Vx: "V x" using disjoint_variables by blast
+      have xmem: "x ∈ set ord" using ord_complete Vx by auto
+      have idx: "find_index ord x < find_index ord v" using topo False by simp
       have idxv: "find_index ord v = length prefix"
         unfolding dec by (rule index_at_split[OF dist])
-      have idx_lt_pref: "find_index ord x < length prefix"
-        using idx idxv by simp
-      have xpref: "x \<in> set prefix"
-      proof -
-        have nthx: "ord ! find_index ord x = x"
-          using find_index_nth_if_mem[OF xmem] .
-        have "prefix ! find_index ord x = x"
-          using nthx idx_lt_pref unfolding dec 
-          by (simp add: nth_append_left)
-        then show ?thesis
-          using idx_lt_pref nth_mem
-          by metis
-      qed
-      have xnot: "x \<notin> set (v # suffix)"
-        using xpref dist by auto
-      have cvx: "cv G x = ?cpre x"
-      proof -
-        have "cv G x = foldl (step_ctx G) (step_ctx G ?cpre v) suffix x"
-          unfolding cv_def dec by simp
-        also have "... = step_ctx G ?cpre v x"
-  using foldl_step_notin xnot by auto
-        also have "... = ?cpre x"
-          using xnot unfolding step_ctx_def by simp
-        finally show ?thesis .
-      qed
-      then show ?thesis
-        by simp
+      have idx_lt_pref: "find_index ord x < length prefix" using idx idxv by simp
+      have xpref: "x ∈ set prefix"
+        using find_index_nth_if_mem[OF xmem] idx_lt_pref
+        by (metis nth_mem nth_append_left dec)
+      have xnot: "x ∉ set (v # suffix)" using xpref dist by auto
+      have "cv G x = foldl (step_ctx G) (step_ctx G ?cpre v) suffix x"
+        unfolding cv_def dec by simp
+      also have "... = ?cpre x"
+        using foldl_step_notin xnot by (simp add: step_ctx_def)
+      finally show ?thesis by simp
     qed
   qed
-  have loc: "G v ?cpre = G v (cv G)"
-    using reachable_locality[OF rG] agree by blast
   show ?thesis
-    using cvv loc by simp
+    using cvv reachable_locality[OF rG] agree by (metis (lifting) ext)
 qed
 
 lemma cv_reachable_fix [simp]:
-  assumes rG: "reachable G"
+  assumes "reachable G"
   shows "Fix G (cv G)"
-  using Fix_iff_solution cv_exo cv_reachable_endo rG by blast
+  using Fix_iff_solution cv_exo cv_reachable_endo assms by blast
 
 lemma fix_agree_endo [simp]:
   assumes rG: "reachable G" and fix1: "Fix G c1" and fix2: "Fix G c2" and Vv: "V v"
   shows "c1 v = c2 v"
   using Vv
-proof (induction v rule: measure_induct_rule[of "\<lambda>v. find_index ord v"])
-  case (less v) 
-  then have Vv: "V v" by simp
-  have c1v: "c1 v = G v c1"
-    using fix1 Vv unfolding Fix_iff_solution by blast
-  have c2v: "c2 v = G v c2"
-    using fix2 Vv unfolding Fix_iff_solution by blast
-  have agree: "\<forall>x. directly_depends v (G v) x \<longrightarrow> c1 x = c2 x"
+proof (induction v rule: measure_induct_rule[of "λv. find_index ord v"])
+  case (less v)
+  have c1v: "c1 v = G v c1" using fix1 less.prems unfolding Fix_iff_solution by blast
+  have c2v: "c2 v = G v c2" using fix2 less.prems unfolding Fix_iff_solution by blast
+  have agree: "∀x. directly_depends v (G v) x ⟶ c1 x = c2 x"
   proof (intro allI impI)
     fix x
     assume dx: "directly_depends v (G v) x"
-    have topo: "U x \<or> find_index ord x < find_index ord v"
-      using reachable_topo_index[OF rG] dx
-      unfolding directly_causes_def by blast
+    have topo: "U x ∨ find_index ord x < find_index ord v"
+      using reachable_topo_index[OF rG] dx unfolding directly_causes_def by blast
     show "c1 x = c2 x"
     proof (cases "U x")
       case True
-      then have "c1 x = tx x"
-        using fix1 unfolding Fix_iff_solution by blast
-      moreover have "c2 x = tx x"
-        using fix2 True unfolding Fix_iff_solution by blast
-      ultimately show ?thesis by simp
+      then show ?thesis
+        using fix1 fix2 unfolding Fix_iff_solution by simp
     next
       case False
-      then have Vx: "V x"
-        using disjoint_variables by blast
-      have "find_index ord x < find_index ord v"
-        using topo False by simp
       then show ?thesis
-        using less.IH[of x] Vx by simp
+        using less.IH[of x] topo disjoint_variables by blast
     qed
   qed
-  have "G v c1 = G v c2"
-    using reachable_locality[OF rG] agree by blast
-  with c1v c2v show ?case by simp
+  show ?case
+    using c1v c2v reachable_locality[OF rG] agree by (smt (verit, best))
 qed
 
 lemma fix_unique [simp]:
-  assumes rG: "reachable G" and fix1: "Fix G c1" and fix2: "Fix G c2"
+  assumes "reachable G" and "Fix G c1" and "Fix G c2"
   shows "c1 = c2"
-  using assms unfolding Fix_iff_solution
-  by (metis (no_types, lifting) ext disjoint_variables fix1 fix2 fix_agree_endo)
+  using assms unfolding Fix_iff_solution 
+  by (metis (no_types, opaque_lifting) assms disjoint_variables ext fix_agree_endo)
 
 lemma reachable_unique_solution [simp]:
-  assumes rG: "reachable G"
-  shows "\<exists>!ctx. Fix G ctx"
-  by (metis cv_reachable_fix fix_unique rG)
+  assumes "reachable G"
+  shows "∃!ctx. Fix G ctx"
+  by (metis cv_reachable_fix fix_unique assms)
 
 lemma cv_eq_if_fix [simp]:
-  assumes rG: "reachable G" and fixc: "Fix G c"
+  assumes "reachable G" and "Fix G c"
   shows "cv G = c"
-  using fixc rG by fastforce
+  using assms by fastforce
 
 lemma cv_intervention_hit [simp]:
   assumes rG: "reachable G" and Yv: "Y v" and Vv: "V v" and Rv: "R v (b v)"
-  shows "cv (update_F G Y b) v = b v" 
+  shows "cv (update_F G Y b) v = b v"
   by (metis Rv Vv Yv cv_reachable_endo rG reachable_step update_F_def wf_intervention_iff)
 
 lemma cv_update_range [simp]:
-  assumes Vv: "V v"
+  assumes "V v"
   shows "R v (cv (update_F F Y b) v)"
   by (metis assms cv_reachable_endo reachable_respects_ranges reachable.simps)
 
 lemma fix_strengthen_intervention [simp]:
-  assumes base: "Fix (update_F F Y b) c"
-      and V1: "V v1" and R1: "R v1 i1" and c1: "c v1 = i1"
+  assumes "Fix (update_F F Y b) c" and "V v1" and "R v1 i1" and "c v1 = i1"
   shows "Fix (update_F F (fun_upd Y v1 True) (fun_upd b v1 i1)) c"
-  using Fix_iff_solution base c1 update_F_def by fastforce
+  using Fix_iff_solution assms update_F_def by fastforce
 
 lemma directly_depends_const [simp]:
-  "\<not> directly_depends v (\<lambda>_. (c :: \<iota>)) x"
+  "¬ directly_depends v (λ_. (c :: ι)) x"
   by simp
 
 end
